cleanq/rb: some lemmas to show write to head does not change any sets
Signed-off-by: Roni Häcki <roni.haecki@inf.ethz.ch>

CleanQ/CleanQ_RBModel.thy
@@ -265,6 +265,7 @@ text \<open>
 definition CleanQ_RB_enq_x :: "'a \<Rightarrow> 'a CleanQ_RB_State  \<Rightarrow> 'a CleanQ_RB_State"
   where "CleanQ_RB_enq_x b rb = rb \<lparr> rSX := (rSX rb) - {b}, rTXY := rb_enq b (rTXY rb) \<rparr>"
 
+
 definition CleanQ_RB_enq_y :: "'a \<Rightarrow> 'a CleanQ_RB_State  \<Rightarrow> 'a CleanQ_RB_State"
   where "CleanQ_RB_enq_y b rb = rb \<lparr> rSY := (rSY rb) - {b}, rTYX := rb_enq b (rTYX rb) \<rparr>"
 
@@ -278,6 +279,17 @@ definition CleanQ_RB_enq_x_possible :: "'a CleanQ_RB_State \<Rightarrow> bool"
 
 definition CleanQ_RB_enq_y_possible :: "'a CleanQ_RB_State \<Rightarrow> bool"
   where "CleanQ_RB_enq_y_possible rb \<longleftrightarrow> rb_can_enq (rTYX rb)"
+
+
+text \<open>
+  Only the write part of enq for concurrency proofs. 
+\<close>
+
+definition CleanQ_RB_enq_write_x :: "'a \<Rightarrow> 'a CleanQ_RB_State  \<Rightarrow> 'a CleanQ_RB_State"
+  where "CleanQ_RB_enq_write_x b rb = rb \<lparr> rSX := (rSX rb), rTXY := rb_write_head b (rTXY rb) \<rparr>"
+
+definition CleanQ_RB_enq_write_y :: "'a \<Rightarrow> 'a CleanQ_RB_State  \<Rightarrow> 'a CleanQ_RB_State"
+  where "CleanQ_RB_enq_write_y b rb = rb \<lparr> rSX := (rSX rb), rTYX := rb_write_head b (rTYX rb) \<rparr>"
 
 
 text \<open>
@@ -882,6 +894,24 @@ lemma CleanQ_RB_deq_y_I4 :
   using can_deq invariants
   by(simp add: CleanQ_RB_deq_y_possible_def rb_deq_remains_valid prod.case_eq_if CleanQ_RB_Invariants_simp) 
 
+
+lemma CleanQ_RB_enq_x_write_I1:
+  assumes Inv:" CleanQ_RB_Invariants K rb" and
+          sx: "b \<in> rSX rb" and
+          enq:"CleanQ_RB_enq_x_possible rb" 
+  shows "CleanQ_RB_list (rTXY (CleanQ_RB_enq_write_x b rb)) = CleanQ_RB_list (rTXY rb)"
+  using assms
+  by (metis CleanQ_RB_State.select_convs(3) CleanQ_RB_State.surjective CleanQ_RB_State.update_convs(3) 
+      CleanQ_RB_enq_write_x_def rb_enq_write_same) 
+
+lemma CleanQ_RB_enq_y_write_I1:
+  assumes Inv:" CleanQ_RB_Invariants K rb" and
+          sy: "b \<in> rSY rb" and
+          enq:"CleanQ_RB_enq_y_possible rb" 
+  shows "CleanQ_RB_list (rTYX (CleanQ_RB_enq_write_y b rb)) = CleanQ_RB_list (rTYX rb)"
+  using assms
+  by (metis CleanQ_RB_State.ext_inject CleanQ_RB_State.surjective CleanQ_RB_State.update_convs(4) CleanQ_RB_enq_write_y_def rb_enq_write_same)
+  
 lemma CleanQ_RB_deq_x_all_inv :
   assumes can_deq: "CleanQ_RB_deq_x_possible rb"  and  X_deq: "rb' = CleanQ_RB_deq_x rb"
     and invariants : "CleanQ_RB_Invariants K rb"
@@ -901,7 +931,6 @@ lemma CleanQ_RB_deq_y_all_inv :
   using can_deq invariants CleanQ_RB_deq_y_I4 CleanQ_RB_deq_y_I3 CleanQ_RB_deq_y_I2 CleanQ_RB_deq_y_I1
   unfolding CleanQ_RB_deq_y_def
   using CleanQ_RB_Invariants_def by fastforce
-
 
 
 (* ==================================================================================== *)
